added operation functions for footprint

rustfrontend/MoveCheckingFootprint1.v
@@ -35,11 +35,13 @@ Inductive footprint : Type :=
 | fp_scalar (ty: type) (v: val)       (* type must be scalar type. *)
 | fp_box (b: block) (sz: Z) (fp: footprint) (* A heap block storing values that occupy footprint fp *)
 (* (field ident, field type, field offset,field footprint) *)
-| fp_struct (id: ident) (fpl: list (ident * Z * footprint))
+| fp_struct (id: ident) (fpl: list (ident * (Z * footprint)))
 (* orgs are not used for now but it is used to relate to the type *)
-| fp_enum (id: ident) (orgs: list origin) (tag: Z) (fid: ident) (ofs: Z) (fp: footprint)
-| fp_ref (ty: type) (phs: paths) (* reference to an owner at [phs] with type [ty] *)
+| fp_enum (id: ident) (* (orgs: list origin) *) (tag: Z) (fid: ident) (ofs: Z) (fp: footprint)
+| fp_ref (b: block) (ofs: Z) (phs: paths) (* reference to an owner at [phs] with type [ty] *)
 .
+
+Definition ffpty : Type := ident * (Z * footprint).
 
 Local Open Scope sep_scope.
 
@@ -63,12 +65,12 @@ Inductive Forall_sep {A : Type} (P : A -> massert -> Prop) : list A -> massert -
 which would report error that sem_wt_loc does not occur positively, so
 we define it here to make sem_wt_loc occurs positively in
 sem_wt_struct case *)
-Inductive fields_sep (b: block) (ofs: Z) (P: footprint -> block -> Z -> massert -> Prop) : list (ident * Z * footprint) -> massert -> Prop :=
+Inductive fields_sep (b: block) (ofs: Z) (P: footprint -> block -> Z -> massert -> Prop) : list ffpty -> massert -> Prop :=
 | fields_sep_nil: fields_sep b ofs P nil STrue
 | fields_sep_cons: forall fid fofs ffp l mass1 mass2
     (IND: fields_sep b ofs P l mass2)
     (FWT: P ffp b (ofs + fofs) mass1),
-    fields_sep b ofs P ((fid, fofs, ffp) :: l) (mass1 ** mass2).
+    fields_sep b ofs P ((fid, (fofs, ffp)) :: l) (mass1 ** mass2).
 
 Section COMP_ENV.
 
@@ -95,17 +97,19 @@ Inductive sem_wt_loc : footprint -> block -> Z -> massert -> Prop :=
 | sem_wt_scalar: forall ty b ofs chunk v
     (MODE: Rusttypes.access_mode ty = Ctypes.By_value chunk),
     sem_wt_loc (fp_scalar ty v) b ofs (hasvalue chunk b ofs v)
+| sem_wt_ref: forall b1 b2 ofs1 ofs2 phs,
+    sem_wt_loc (fp_ref b2 ofs2 phs) b1 ofs1 (hasvalue Mptr b1 ofs1 (Vptr b2 (Ptrofs.repr ofs2)))
 | sem_wt_box: forall b ofs fp b1 sz1 v mass
     (WTVAL: sem_wt_val (fp_box b1 sz1 fp) v mass),
     sem_wt_loc (fp_box b1 sz1 fp) b ofs ((hasvalue Mptr b ofs v) ** mass)
 | sem_wt_struct: forall b ofs fpl id mass
     (FWT: fields_sep b ofs sem_wt_loc fpl mass),
     sem_wt_loc (fp_struct id fpl) b ofs mass
-| sem_wt_enum: forall fp b ofs tagz fid fofs id orgs mass1 mass2
+| sem_wt_enum: forall fp b ofs tagz fid fofs id mass1 mass2
     (* Interpret the field by the tag and prove that it is well-typed *)
     (TAG: mass1 = hasvalue Mint32 b ofs (Vint (Int.repr tagz)))
     (FWT: sem_wt_loc fp b (ofs + fofs) mass2),
-    sem_wt_loc (fp_enum id orgs tagz fid fofs fp) b ofs (mass1 ** mass2)
+    sem_wt_loc (fp_enum id tagz fid fofs fp) b ofs (mass1 ** mass2)
 
 
 with sem_wt_val : footprint -> val -> massert -> Prop :=
@@ -114,9 +118,11 @@ with sem_wt_val : footprint -> val -> massert -> Prop :=
 | wt_val_box: forall b fp sz mass1 mass2
     (WTLOC: sem_wt_loc fp b 0 mass1)
     (** TODO: support negative range  *)
-    (MASS: mass2 = range b (- size_chunk Mptr) sz
-                   ** contains_neg Mptr b (- size_chunk Mptr) (eq (Vptrofs (Ptrofs.repr sz)))
-                   ** mass1)
+    (MASS: mass2 = (mconj (range b (- size_chunk Mptr) sz)
+                      (* note that (-8, sz) is overlapped with mass1
+                      and the following contains_neg*)
+                      ((contains_neg Mptr b (- size_chunk Mptr) (eq (Vptrofs (Ptrofs.repr sz)))))
+                      ** mass1))
     (* sz > 0 is used to make sure extcall_ext_free succeeds and sz <=
     max_unsigned is used to provent overflow when traversing some
     field offsets *)
@@ -133,11 +139,11 @@ with sem_wt_val : footprint -> val -> massert -> Prop :=
     (PERM: mass2 = range b (Ptrofs.unsigned ofs) (Ptrofs.unsigned ofs + sizeof_comp id)),
     (** mass1 and mass2 are overlapped!! *)
     sem_wt_val (fp_struct id fpl) (Vptr b ofs) (mconj mass1 mass2)
-| wt_val_enum: forall b ofs fp tagz fid fofs id orgs mass1 mass2
-    (WTLOC: sem_wt_loc (fp_enum id orgs tagz fid fofs fp) b (Ptrofs.unsigned ofs) mass1)
+| wt_val_enum: forall b ofs fp tagz fid fofs id mass1 mass2
+    (WTLOC: sem_wt_loc (fp_enum id tagz fid fofs fp) b (Ptrofs.unsigned ofs) mass1)
     (AL: (alignof_comp id | Ptrofs.unsigned ofs))
     (PERM: mass2 = range b (Ptrofs.unsigned ofs) (Ptrofs.unsigned ofs + sizeof_comp id)),
-    sem_wt_val (fp_enum id orgs tagz fid fofs fp) (Vptr b ofs) (mconj mass1 mass2).
+    sem_wt_val (fp_enum id tagz fid fofs fp) (Vptr b ofs) (mconj mass1 mass2).
 
 
 
@@ -147,9 +153,9 @@ Variable (P: footprint -> Prop)
   (HPemp: P fp_emp)
   (HPscalar: forall ty v, P (fp_scalar ty v))
   (HPbox: forall (b : block) sz (fp : footprint), P fp -> P (fp_box b sz fp))
-  (HPstruct: forall id fpl, (forall fid ofs fp, In (fid, ofs, fp) fpl -> P fp) -> P (fp_struct id fpl))
-  (HPenum: forall id orgs (tag : Z) fid ofs (fp : footprint), P fp -> P (fp_enum id orgs tag fid ofs fp))
-  (HPref: forall ty ref_owner, P (fp_ref ty ref_owner)).
+  (HPstruct: forall id fpl, (forall fid ofs fp, In (fid, (ofs, fp)) fpl -> P fp) -> P (fp_struct id fpl))
+  (HPenum: forall id (tag : Z) fid ofs (fp : footprint), P fp -> P (fp_enum id tag fid ofs fp))
+  (HPref: forall b ofs ref_owner, P (fp_ref b ofs ref_owner)).
 
 Fixpoint strong_footprint_ind t: P t.
 Proof.
@@ -159,7 +165,7 @@ Proof.
   - eapply HPbox. specialize (strong_footprint_ind t); now subst.
   - eapply HPstruct. induction fpl.
     + intros. inv H.
-    + intros. destruct a as ((fid1 & ofs1) & fp1).  simpl in H. destruct H.
+    + intros. destruct a as (fid1 & ofs1 & fp1).  simpl in H. destruct H.
       * specialize (strong_footprint_ind fp1). inv H. apply strong_footprint_ind.
         (* now subst. *)
       * apply (IHfpl fid ofs fp H). 
@@ -178,12 +184,12 @@ Fixpoint footprint_flat (fp: footprint) : flat_footprint :=
   match fp with
   | fp_emp => nil
   | fp_scalar _ _ => nil
-  | fp_ref _ _ => nil
+  | fp_ref _ _ _ => nil
   | fp_box b _ fp' =>
       b :: footprint_flat fp'
   | fp_struct _ fpl =>
-      flat_map (fun '(_, _, fp) => footprint_flat fp) fpl
-  | fp_enum _ _ _ _ _ fp =>
+      flat_map (fun '(_, (_, fp)) => footprint_flat fp) fpl
+  | fp_enum _ _ _ _ fp =>
       footprint_flat fp
   end.
 
@@ -212,6 +218,8 @@ Definition flat_fp_map (fpm: fp_map) : flat_footprint :=
 
 (* Definiton of footprint for stack frames *)
 
+Definition fenv := PTree.t (block * Z * type).
+
 (** Footprint map which records the footprint starting from stack
 blocks (denoted by variable names). It represents the ownership chain
 from a stack block. *)
@@ -220,8 +228,10 @@ from a stack block. *)
 
 Inductive fp_frame : Type :=
 | fpf_emp
-(* we need to record the footprint of the stack *)
-| fpf_func (e: env) (fpm: fp_map) (fpf: fp_frame)
+(* we need to record the footprint of the stack. Can we just use one
+local environment to record the location of local variables and
+locations passed by reference from the caller? *)
+| fpf_func (e: fenv) (fpm: fp_map) (fpf: fp_frame)
 (* use this to record the structure of footprint in dropplace state, rfp is the footprint of the place being dropped *)
 (** We may not need fpf_dropplace. We can prove some invariant for the
 places in drop_place_state, e.g., their footprint in fpm is not
@@ -230,18 +240,20 @@ shallowly fp_emp and etc. *)
 (* record the footprint in a drop glue: fpl are the footprint of the
 members to be dropped (the first element of fpl is the current dropped
 footprint); (b, ofs) is the address of this composite. *)
-| fpf_drop (b: block) (ofs: Z) (fpl: list (ident * Z * footprint)) (fpf: fp_frame)
+| fpf_drop (b: block) (ofs: Z) (fpl: list (ffpty)) (fpf: fp_frame)
 .
 
-Inductive coherent_var (fpm: fp_map) (elt: (ident * (block * type))) : massert -> Prop :=
-| coherent_var_intro: forall id b ty mass fp
-    (ELTEQ: elt = (id, (b, ty)))
+Inductive coherent_var (fpm: fp_map) (elt: (ident * (block * Z * type))) : massert -> Prop :=
+| coherent_var_intro: forall id b ofs ty mass fp
+    (ELTEQ: elt = (id, (b, ofs, ty)))
+    (* What if fpm contains more variables than local env? *)
     (VARFP: fpm ! id = Some fp)
     (MASS: sem_wt_loc fp b 0 mass),
-    coherent_var fpm elt mass.
+    (* local variables are freeable (defined by range) *)
+    coherent_var fpm elt (mconj mass (range b ofs (sizeof ce ty))).
 
 (* The separation predicate for (local env, footprint map) *)
-Inductive coherent_fpm (e: env) (fpm: fp_map) : massert -> Prop :=
+Inductive coherent_fpm (e: fenv) (fpm: fp_map) : massert -> Prop :=
 | coherent_fpm_intro: forall mass
     (ALLSEP: Forall_sep (coherent_var fpm) (PTree.elements e) mass),
     coherent_fpm e fpm mass.
@@ -266,4 +278,337 @@ Inductive coherent (m: mem) (fpf: fp_frame) : Prop :=
     (MPRED: m |= mass),
     coherent m fpf.
 
-(** Next step:   *)
+End COMP_ENV.
+
+(** Functions for getting and updating the footprint map. *)
+
+(* [set_footprint] and [set_footprint_map] set some footprint [fp] to
+the path (id, phl); [get_footprint] gets footprint from a footprint
+with a path and [get_loc_footprint_map] gets footprint and the
+location storing this footprint; [clear_footprint(_map)] set the
+footprint at the path [phl] to fp_emp; We also need to distinguish
+getting footprint through owner path and arbitary path (i.e., paths
+containing dereference reference), so we define [get_footprint(_map)
+to get the footprint from arbitary path which uses a function
+[get_owner_loc_footprint_(map)]] which gets footprint from only owner
+paths. This distinguishment may not be needed for set functions as we
+can ensure that we only set owner paths?  *)
+
+(** TODO: it would be better to use list_find and its properties from stdpp. *)
+Definition find_field {A: Type} (id: ident) (l: list (ident * A)) : option (ident * A) :=
+  find (fun '(id', _) => if ident_eq id id' then true else false) l. 
+
+Definition field_idents {A: Type} (l: list (ident * A)) : list ident :=
+  map (fun '(fid, _) => fid) l.
+
+(* only set the first occurence of fid *)
+Fixpoint set_field {A: Type} (id: ident) (f: A -> A) (l: list (ident * A)) : list (ident * A) :=
+  match l with
+  | nil => nil
+  | (id', a') :: l' =>
+      if ident_eq id id' then
+        (id, f a') :: l'
+      else
+        (id', a') :: (set_field id f l')
+  end.
+
+Definition set_field_fp (fid: ident) (vfp: footprint) (fpl: list (ffpty)) : list ffpty :=
+  set_field fid (fun '(fofs, ffp) => (fofs, vfp)) fpl.
+
+(* set footprint [v] in the path [ph] of footprint [fp] *)
+Fixpoint set_footprint (phl: list path) (v: footprint) (fp: footprint) : option footprint :=
+  match phl with
+  | nil => Some v
+  | ph :: l =>
+      match ph, fp with
+      | ph_deref, fp_box b sz fp1 =>
+          match set_footprint l v fp1 with
+          | Some fp2 =>
+              Some (fp_box b sz fp2)
+          | None => None
+          end
+      | ph_field fid, fp_struct id fpl =>
+          match find_field fid fpl with
+          | Some (fid1, (fofs, ffp)) =>
+              match set_footprint l v ffp with
+              | Some ffp1 =>
+                  Some (fp_struct id (set_field_fp fid ffp1 fpl)) 
+              | None => None
+              end
+          | None => None
+          end
+      (* TODO: remove pty in ph_downcast *)
+      | ph_downcast _ fid (* fty *), fp_enum id tagz fid1 fofs1 fp1 =>
+          (** Type safe checking *)
+          if ident_eq fid fid1 then
+            match set_footprint l v fp1 with
+            | Some fp2 =>
+                Some (fp_enum id tagz fid1 fofs1 fp2)
+            | None => None
+            end
+          else None
+      | _, _ => None
+      end
+  end.
+
+Definition set_footprint_map (ps: paths) (v: footprint) (fpm: fp_map) : option fp_map :=
+  let (id, phl) := ps in
+  match fpm!id with
+  | Some fp1 =>
+      match set_footprint phl v fp1 with
+      | Some fp2 =>
+          Some (PTree.set id fp2 fpm)
+      | None =>
+          None
+      end
+  | None => None
+  end.
+
+
+Fixpoint get_owner_loc_footprint (phl: list path) (fp: footprint) (b: block) (ofs: Z) : option (block * Z * footprint) :=
+  match phl with
+  | nil => Some (b, ofs, fp)
+  | ph :: l =>
+      match ph, fp with
+      | ph_deref, fp_box b _ fp1 =>
+          get_owner_loc_footprint l fp1 b 0
+      | ph_field fid, fp_struct _ fpl =>
+          match find_field fid fpl with
+          | Some (_, (fofs, fp1)) =>
+              get_owner_loc_footprint l fp1 b (ofs + fofs)
+          | None => None
+          end
+      | ph_downcast _ fid1 (* fty1 *), fp_enum id _ fid2 fofs fp1 =>
+          if ident_eq fid1 fid2  then
+            get_owner_loc_footprint l fp1 b (ofs + fofs)
+          else None
+      | _, _  => None
+      end
+  end.
+
+(* non-loc version: use it to get some internal footprint *)
+Fixpoint get_owner_footprint (phl: list path) (fp: footprint) : option footprint :=
+  match phl with
+  | nil => Some fp
+  | ph :: l =>
+      match ph, fp with
+      | ph_deref, fp_box b _ fp1 =>
+          get_owner_footprint l fp1
+      | ph_field fid, fp_struct _ fpl =>
+          match find_field fid fpl with
+          | Some (_, (fofs, fp1)) =>
+              get_owner_footprint l fp1
+          | None => None
+          end
+      | ph_downcast pty fid1 (* fty1 *), fp_enum id _ fid2 fofs fp1 =>
+          if ident_eq fid1 fid2 then
+            get_owner_footprint l fp1
+          else
+            None
+      | _, _  => None
+      end
+  end.
+
+
+Definition get_owner_loc_footprint_map (e: fenv) (ps: paths) (fpm: fp_map) : option (block * Z * footprint) :=
+  let (id, phl) := ps in
+  match e!id, fpm!id with
+  | Some (b, ofs, ty), Some fp =>
+      get_owner_loc_footprint phl fp b ofs
+  | _, _ => None
+  end.
+
+Fixpoint clear_footprint_rec (fp: footprint) : footprint :=
+  match fp with
+  | fp_scalar _ _
+  | fp_box _ _ _
+  | fp_enum _ _ _ _ _
+  | fp_ref _ _ _
+  | fp_emp => fp_emp
+  | fp_struct id fpl =>
+      fp_struct id (map (fun '(fid, (fofs, ffp)) => (fid, (fofs, clear_footprint_rec ffp))) fpl)
+  end.
+
+Definition clear_footprint_map (e: fenv) (ps: paths) (fpm: fp_map) : option fp_map :=
+  match get_owner_loc_footprint_map e ps fpm with
+  | Some (_, _, fp1) =>
+      set_footprint_map ps (clear_footprint_rec fp1) fpm
+  | None => None
+  end.
+
+(* Get location and footprint through paths which may contains
+dereference of reference *)
+
+Fixpoint get_loc_footprint (fe: fenv) (fpm: fp_map) (phl: list path) (fp: footprint) (b: block) (ofs: Z) : option (block * Z * footprint) :=
+  match phl with
+  | nil => Some (b, ofs, fp)
+  | ph :: l =>
+      match ph, fp with
+      | ph_deref, fp_box b _ fp1 =>
+          get_owner_loc_footprint l fp1 b 0
+      | ph_field fid, fp_struct _ fpl =>
+          match find_field fid fpl with
+          | Some (_, (fofs, fp1)) =>
+              get_loc_footprint fe fpm l fp1 b (ofs + fofs)
+          | None => None
+          end
+      | ph_downcast _ fid1 (* fty1 *), fp_enum id _ fid2 fofs fp1 =>
+          if ident_eq fid1 fid2  then
+            get_loc_footprint fe fpm l fp1 b (ofs + fofs)
+          else None
+      | ph_deref, fp_ref b1 ofs1 phs1 =>
+          match get_owner_loc_footprint_map fe phs1 fpm with
+          | Some (b2, ofs2, fp2) =>
+              (* If this reference is valid, (b1, ofs1) should be
+              equal to (b2, ofs2) *)
+              get_loc_footprint fe fpm l fp2 b2 ofs2
+          | None => None
+          end
+      | _, _  => None
+      end
+  end.
+
+Definition get_loc_footprint_map (fe: fenv) (ps: paths) (fpm: fp_map) : option (block * Z * footprint) :=
+  let (id, phl) := ps in
+  match fe!id, fpm!id with
+  | Some (b, ofs, ty), Some fp =>
+      get_loc_footprint fe fpm phl fp b ofs
+  | _, _ => None
+  end.
+
+
+(** ** Typing of the footprint: used to make sure the footprint is well-formed *)
+
+
+Section COMP_ENV.
+
+Variable ce: composite_env.
+
+Fixpoint wt_path (ty: type) (phl: list path) : res type :=
+  match phl with
+  | nil => OK ty
+  | ph :: phl1 =>
+      do ty1 <- 
+           match ph with
+           | ph_deref => type_deref ty
+           | ph_field fid => type_field ce ty fid
+           | ph_downcast _ fid => type_downcast ce ty fid
+           end;
+      wt_path ty1 phl1
+  end.
+
+
+(* Definition of wt_footprint (well-typed footprint). Intuitively, it
+says that the footprint is an abstract form of the syntactic type. *)
+Inductive wt_footprint : type -> footprint -> Prop :=
+| wt_fp_emp: forall ty
+    (* It means that the location with this type is not initialized or
+        this location is scalar type. We require that [ty] is not
+        structure because we do not want to dynamically unpack the
+        struct when setting footprint (e.g., by set_loc_footprint) to
+        some field of this struct. But to ensure this properties, we
+        need to carefully set fp_emp to place with structure type. *)
+    (WF: forall orgs id, ty <> Tstruct orgs id),
+    wt_footprint ty fp_emp
+| wt_fp_scalar: forall ty v
+    (WF: scalar_type ty = true),
+    wt_footprint ty (fp_scalar ty v)
+| wt_fp_struct: forall orgs id fpl co
+    (CO: ce ! id = Some co)
+    (STRUCT: co_sv co = Struct)
+    (** TODO: combine WT1 andp WT2 elegantly. WT1 is used in getting
+    the sub-field's footprint. WT2 is used in proving the properties
+    of sub-field's footprint *)
+    (WT1: forall fid fty,
+        place_field_type co fid orgs = OK fty ->
+        (* For simplicity, use find_field instead of In predicate *)
+        exists ffp fofs,
+          find_field fid fpl = Some (fid, (fofs, ffp))
+          /\ field_offset ce fid co.(co_members) = OK fofs
+          (* bound condition *)
+          /\ wt_footprint fty ffp)
+    (WT2: forall fid fofs ffp,
+        find_field fid fpl = Some (fid, (fofs, ffp)) ->
+        exists fty,
+          place_field_type co fid orgs = OK fty
+          /\ field_offset ce fid co.(co_members) = OK fofs
+          /\ wt_footprint fty ffp)
+    (* make sure that the flattened footprint list has the same order
+    as that of the members. If we can ensure that name_members are
+    norepeated, then so are the field_idents. *)
+    (FLAT: field_idents fpl = name_members (co_members co)),
+    wt_footprint (Tstruct orgs id) (fp_struct id fpl)
+| wt_fp_enum: forall orgs id tagz fid fty fofs fp co
+    (CO: ce ! id = Some co)
+    (ENUM: co_sv co = TaggedUnion)
+    (TAG: list_nth_z co.(co_members) tagz = Some (Member_plain fid fty))
+    (* avoid some norepet properties *)
+    (FTY: place_field_type co fid orgs = OK fty)
+    (FOFS: variant_field_offset ce fid co.(co_members) = OK fofs)
+    (WT: wt_footprint fty fp),
+    wt_footprint (Tvariant orgs id) (fp_enum id tagz fid fofs fp)
+| wt_fp_box: forall ty b fp
+    (* this is ensured by bm_box *)
+    (WT: wt_footprint ty fp),
+    (* It is used to make sure that dropping any location within a
+    block does not cause overflow *)
+    wt_footprint (Tbox ty) (fp_box b (sizeof ce ty) fp)
+| wt_fp_ref: forall ty b ofs phs org mut,
+    (** Do we need to prove that phs is well-typed path? *)
+    wt_footprint (Treference org mut ty) (fp_ref b ofs phs).
+
+Definition wt_footprint_list tyl fpl :=
+  list_forall2 wt_footprint tyl fpl.
+
+End COMP_ENV.
+
+
+(** Initialize a footprint with fp_emp based on the type of this footprint *)
+
+Definition members_to_fields_fp_emp ce (ms: members) (f: type -> footprint): list ffpty :=
+  map (fun '(Member_plain fid fty) =>
+         match field_offset ce fid ms with
+         | OK fofs =>
+             (fid, (fofs, f fty))
+         | Error _ => (* we can prove that it is impossible *)
+             (fid, (0, fp_emp))
+         end) ms.
+
+Fixpoint type_to_empty_footprint_rec (ce: composite_env) (rank: nat) (ty: type) : footprint :=
+  match rank with
+  | O => fp_emp
+  | S r =>      
+      match ty with
+      | Tstruct _ id =>
+          match ce ! id with
+          | Some co =>
+              let fields := members_to_fields_fp_emp ce (co_members co) (type_to_empty_footprint_rec ce r) in
+              fp_struct id fields
+          | None => fp_emp
+          end
+      | _ => fp_emp
+      end
+  end.
+
+Definition type_to_empty_footprint (ce: composite_env) (ty: type) : footprint :=
+  type_to_empty_footprint_rec ce (rank_type ce ty) ty.
+
+Lemma type_to_empty_footprint_rec_eq: forall ce ty1 ty2,
+    type_eq_except_origins ty1 ty2 = true ->
+    type_to_empty_footprint_rec ce (rank_type ce ty1) ty1 = type_to_empty_footprint_rec ce (rank_type ce ty2) ty2.
+Admitted.
+
+Lemma type_to_empty_footprint_eq: forall ce ty1 ty2,
+    type_eq_except_origins ty1 ty2 = true ->
+    type_to_empty_footprint ce ty1 = type_to_empty_footprint ce ty2.
+Proof.
+  intros. eapply type_to_empty_footprint_rec_eq. auto.
+Qed.
+
+(** We need that ce is consistent so that if ty is struct then ce
+contains this struct *)
+Lemma type_to_empty_footprint_wt: forall ce ty,
+    complete_type ce ty = true ->
+    wt_footprint ce ty (type_to_empty_footprint ce ty).
+Admitted.
+
